 #PureMath #Study 
#### What is the derivative of $Y= f(x)$
 $y'$ , $f'(x)$, $\frac{dy}{dx}$, $\frac{d}{dx}(f(x))$ are the all derivative of $Y= f(x)$
 
 ### Some Rules:
1. $f(x) = a ε R$  where a is constant (independent on x ) => $f'(x) = 0$
2. $f(x) = {x^{n}}, n ε R => f'(x) = {nx^{n-1}}$
3. $f(x) = x => f'(x) = 1$
4. $\frac{a}{x^{n}} = a{x^{-n}}$
5. $f(x) = \sqrt[n]{x} = {{x}^\frac{1}{n}}$

### Explanation of Differentiation Rules

1. **Constant Function**  
    **Rule:**  If $f(x)=a$ (where a is a constant), then $f′(x)=0f′(x)=0.$
    **Explanation:** The derivative measures the rate of change. Since a constant does not change, its slope is zero.  
    **Example:**
$$
    f(x)=5⇒f′(x)=0
$$
2. **Power Rule**  
    **Rule:** If  $f(x) = {x^{n}}, n ε R => f'(x) = {nx^{n-1}}$
    **Explanation:** The exponent $n$ moves to the front, and the new exponent becomes $n−1$. Applies to all real numbers $n$, but assumes $x>0$ for irrational/fractional exponents.  
    **Example:**
$$
	f(x)= {x^{3}}⇒f'(x) =1
$$
3. **Linear Function**  
    **Rule:** If $f(x) = x => f'(x) = 1$
    **Explanation:** This is a special case of the power rule where $n=1$. The slope of $f(x)=x$ is 1 everywhere.  
    **Example:**
    
$$
    f(x)=x⇒f′(x)=1
$$
4. **Negative Exponents**  
    **Rule:** $\frac{a}{x^{n}} = a{x^{-n}}$ 
    **Explanation:** Rewrite expressions with denominators to use the power rule.  
    **Example:**
    
$$
    f(x)=\frac{4}{x^{2}}={4x^{−2}}⇒f′(x)=4(−2){x^{−3}}=\frac{-8}{x^{3}}​
$$
5. **Roots as Exponents**  
    **Rule:** $f(x) = \sqrt[n]{x} = {{x}^\frac{1}{n}}$
    **Explanation:** Convert roots to fractional exponents to apply the power rule.  
    **Example:**
    $$
    f(x) = \sqrt{x} = x^{\frac{1}{2}} ⇒ f'(x) = \frac{1}{2}x^{\frac{-1}{2}} = \frac{1}{2\sqrt{x}} 
    $$


---

### Key Notes:

- **Negative/Fractional Exponents:** Handle signs and fractions carefully to avoid errors.
    
- **Differentiability:** Rules assume xx is in the domain (e.g., x>0x>0 for x13x31​).
    
- **Common Mistakes:**
    
    - Forgetting to reduce the exponent by 1.
        
    - Misapplying the rule to constants (e.g.,$\frac{d}{dx}[5] not = 5$
        

**Example Summary:**
$f(x)=3^{x4}−\frac{2}{x}​+7=>3^x{4}−2x^{−1}+7$
$f′(x)=12x^{3}+2x^{−2}=12x^{3}+\frac{2}{x^{2}}​​$

==These rules form the foundation for differentiating polynomial and rational functions.==
