#PureMath #Study 

**Product Rule:**  
If $y = f(x) \cdot g(x)$, then:  

$$
\frac{dy}{dx} = f(x) \cdot g'(x) + g(x) \cdot f'(x)
 
$$
---

## Example 1:  
**Function:** ( $y = (3x^2 - 2x + 1)(x^4 - 5x^2 + 2)$ at $x = 0$ .  

### Steps:  
1. **Identify \( f(x) \) and \( g(x) \):**  
   
$$
   f(x) = 3x^2 - 2x + 1, \quad g(x) = x^4 - 5x^2 + 2
$$

2. **Compute derivatives:**  

$$
   f'(x) = 6x - 2, \quad g'(x) = 4x^3 - 10x
$$

3. **Apply the product rule:**  

$$
   \frac{dy}{dx} = (3x^2 - 2x + 1)(4x^3 - 10x) + (x^4 - 5x^2 + 2)(6x - 2)
$$

4. **Substitute \( x = 0 \):**  

$$
   \frac{dy}{dx} = (1)(0) + (2)(-2) = -4
$$


**Result:**  

$$
\boxed{-4}
$$


---

## Example 2:  
**Function:** \( $y = (2x + 5)(3x^2 - 1$) \) at \( $x = -1$ \).  

### Steps:  
1. **Identify \( f(x) \) and \( g(x) \):**  

$$
   f(x) = 2x + 5, \quad g(x) = 3x^2 - 1
$$

2. **Compute derivatives:**  
   
$$
   f'(x) = 2, \quad g'(x) = 6x
$$

3. **Apply the product rule:**  
   
$$
   \frac{dy}{dx} = (2x + 5)(6x) + (3x^2 - 1)(2)
$$
   
4. **Substitute \( x = -1 \):**  
   
   $\frac{dy}{dx} = (3)(-6) + (2)(2) = -18 + 4 = -14$
   

**Result:**  

$\boxed{-14}$

---

## Key Takeaways:  
- **Product Rule Formula:**  

$$
  \frac{d}{dx}[f \cdot g] = f \cdot g' + g \cdot f'
$$

- **Critical Steps:**  
  - Differentiate \( f(x) \) and \( g(x) \) separately.  
  - Substitute values **after** differentiating.  
- **Common Errors:**  
  - Misapplying signs (e.g., at \( x = -1 \)).  
  - Forgetting to multiply terms correct