**Equation of a Normal Line**  

---

### Formula:  
Normal line is **perpendicular** to the tangent.  
If $m$ is the slope of the tangent, then slope of normal is $-\frac{1}{m}$  

Equation:  
$$
y - f(a) = -\frac{1}{f'(a)}(x - a)
$$  

---

### Example:  
**Function:** $y = x^2$ at $x = 2$  

1. **From tangent example:**  
   $f(2) = 4$, $f'(2) = 4$  

2. **Normal slope:**  
   $m = -\frac{1}{4}$  

3. **Equation:**  
   $$
   y - 4 = -\frac{1}{4}(x - 2)
   $$  
   $$
   \Rightarrow y = -\frac{1}{4}x + \frac{1}{2} + 4 = -\frac{1}{4}x + \frac{9}{2}
   $$  

**Result:**  
$$
\boxed{y = -\frac{1}{4}x + \frac{9}{2}}
$$  

---

### Tip:  
Tangent and normal intersect at the same point on the curve, but have **perpendicular slopes**.
